\documentclass[12pt]{article}
\usepackage{amsmath}

\begin{document}

%https://latexbase.com
    \[\frac{rc_0}{rc_1}x = \frac{-rc_1}{rc_0}\left(x-v_0\right)+v_1\]
    \[\frac{rc_0}{rc_1}x = \frac{-rc_1\left(x-v_0\right)}{rc_0}+v_1\]
    \[\frac{rc_0}{rc_1}x = \frac{-rc_1x+rc_1v_0}{rc_0}+v_1\]
    \[\frac{{rc_0}^2}{rc_1}x = -rc_1x+rc_1v_0+v_1rc_0\]
    \[{rc_0}^2x = -{rc_1}^2x+{rc_1}^2v_0+v_1rc_0rc_1\]
    \[{rc_0}^2x+{rc_1}^2x = {rc_1}^2v_0+v_1rc_0rc_1\]
    \[\left({rc_0}^2+{rc_1}^2\right)x = {rc_1}^2v_0+v_1rc_0rc_1\]
    \[x = \frac{{rc_1}^2v_0+v_1rc_0rc_1}{{rc_0}^2+{rc_1}^2}\]

\end{document}
